Add most for initial version of term specialization

generic.v
@@ -2,17 +2,13 @@ Set Implicit Arguments.
 
 Require Import univ utils.
 
-Require Import Nat.
+From Coq Require Import Nat.
 
 (* Generic Library *)
 
 (** Still mostly just playing around, this is basically a combination of ideas
   from 'Arity-Generic Datatype-Generic Programming' and
   'Polytypic Programming in Coq'. **)
-
-Record PolyType (n : nat) : Type := polyType {
-typeKindStar : nary_fn n Set Set
-}.
 
 (****** Type specialization ******)
 
@@ -25,39 +21,25 @@ typeKindStar : nary_fn n Set Set
 (* so b is literally the way to construct the type of the operation
       e.g. Map : vec Set 2 -> Set
       Map (A :: B :: []) = A -> B *)
-Fixpoint kit (n : nat) (k : kind) (b : vec Set n -> Set)
-  : vec (decodeKind k) n -> Set :=
-    match k return vec (decodeKind k) n -> Set with
+Fixpoint kit (n : nat) (k : kind) (b : vec Set (S n) -> Set)
+  : vec (decodeKind k) (S n) -> Set :=
+    match k return vec (decodeKind k) (S n) -> Set with
     | Ty => fun vs => b vs
     | F k1 k2 => fun vs => quantify (fun As => kit k1 b As ->
                                                kit k2 b (zap vs As))
-    end.
-
-(* kit (kind-indexed type) for tuples *)
-Fixpoint kit' (n : nat) (k : kind) (pt : PolyType n)
-  : tupleT (decodeKind k) n -> decodeKind Ty :=
-    match k return tupleT (decodeKind k) n -> decodeKind Ty with
-    | Ty => uncurry _ _ _ (typeKindStar pt)
-    | F k1 k2 => fun tup => quantifyT _ _ (fun As => kit' k1 pt As ->
-                                                kit' k2 pt (zapT _ _ _ tup As))
     end.
 
 (* some map examples: *)
 Definition Map : vec Set 2 -> Set :=
   fun vs => vhd vs -> vhd (vtl vs).
 
-Definition MapT : PolyType 2 :=
-  polyType 2 (fun A B => A -> B).
-
 Definition vect (A B : Set) := vcons A (vcons B (vnil _)).
-Definition tupt := (unit, (nat, tt)).
 
 Compute kit Ty Map (vect nat unit). (* = nat -> unit *)
-Compute kit' Ty MapT tupt. (* = unit -> nat *)
 
 (* type for mapping constants to a value *)
 Definition tyConstEnv (n : nat) (b : vec Set (S n) -> Set) : Set :=
-  forall (k:kind) (c:const k), kit k b (repeat _ (decodeClosed _ (Con _ _ c))).
+  forall (k:kind) (c:const k), kit k b (repeat _ (decodeClosed (Con _ c))).
 
 (* helper for mapConst *)
 Definition doSum (A1 B1 : Set)
@@ -77,16 +59,201 @@ Definition doProd (A1 B1 : Set)
 (* Example of building a function for mapping constants to a value. *)
 Definition mapConst : tyConstEnv Map :=
   fun k c =>
-    match c in const k return kit _ Map (repeat _ (decodeClosed _ (Con _ _ c))) with
+    match c in const k return kit _ Map (repeat _ (decodeClosed (Con _ c))) with
     | Nat => fun n => n
     | Unit => fun _ => tt
     | Prod => doProd
     | Sum => doSum
     end.
 
-(* examples of using mapConst *)
-Compute mapConst Prod unit bool (fun _ => true) nat nat (fun b => b + 1) (tt,2).
-Compute mapConst Sum _ _ (fun _ => true)
-                     _ _ (fun n => if eqb n 1 then true else false) (inr 2).
+Definition owng (n : nat) (b : vec Set (S n) -> Set) (ce : tyConstEnv b)
+  (k : kind) (c : const k) :=
+  ce _ c .
+
+(* works only for constants. *)
+Definition cmap := owng mapConst.
+
+Compute cmap Prod _ _ (fun _ => true) _ _ (fun b => b + 1) (tt,2).
+Compute cmap Sum _ _ (fun _ => true)
+                 _ _ (fun n => if eqb n 1 then true else false) (inr 2).
 
 (* Now what is left is term specialization and then done for type-genericity *)
+
+Section terms.
+ (* section for term specialization *)
+
+  (* NGENV *)
+  Inductive ngenv (n : nat) : (vec Set (S n) -> Set) -> ctx -> Type :=
+    | nnil : forall b, ngenv b nil
+    | ncons : forall b (k:kind) (G : ctx) (a : vec (decodeKind k) (S n)),
+        kit k b a -> ngenv b G -> ngenv b (cons k G).
+
+  (* interpret a generic type + vector of envs to a vec of types *)
+  Definition interp' (G : ctx) (k : kind) (n : nat)
+    : typ G k -> vec (env G) n -> vec (decodeKind k) n :=
+    fun t vs =>
+      zap (repeat _ (decodeType t)) vs.
+
+  Definition eqkit : forall (n : nat) (k : kind) (b : vec Set (S n) -> Set)
+    (t1 t2 : vec (decodeKind k) (S n)),
+    t1 = t2 -> kit k b t1 -> kit k b t2.
+  Proof.
+    intros. rewrite <- H; assumption.
+  Qed.
+
+  (* bunch of ngenvs to a vector of envs *)
+  (* use '@' to provide implicits explicitly *)
+  Fixpoint transpose (n : nat) (b : vec Set (S n) -> Set) (G : ctx) (nge : ngenv b G)
+    : vec (env G) (S n) :=
+      match nge with
+      | nnil _ => repeat _ enil
+      | ncons _ a _ nge => zap (zap (repeat _ (@econs _ _)) a) (transpose nge)
+      end.
+
+  (* PROOFS to help with term specialization, definitions from W + C *)
+
+  Lemma eqtail : forall {A} (n : nat) (t1 t2 : vec A n) (x : A),
+    t1 = t2 -> vcons x t1 = vcons x t2.
+  Proof.
+    intros A n t1 t2 x eq. rewrite eq. reflexivity.
+  Qed.
+
+  Lemma c6 : forall (n : nat) (A B : Type) (f : A -> B) (x : A),
+    zap (repeat n f) (repeat n x) = repeat n (f x).
+  Proof.
+    intros n A B f x. induction n.
+    - simpl. reflexivity.
+    - simpl. rewrite IHn. reflexivity.
+  Qed.
+
+  Lemma c5 : forall (n : nat) (k : kind) (G : ctx) (c : const k)
+    (envs : vec (env G) n),
+      repeat n (decodeClosed (Con _ c)) = interp' (Con _ c) envs.
+  Proof.
+    intros n k G c envs. induction envs.
+    - simpl. destruct G.
+      + simpl. reflexivity.
+      + simpl. reflexivity.
+    - simpl. rewrite IHenvs. destruct G.
+      + simpl. reflexivity.
+      + simpl. reflexivity.
+  Qed.
+
+  Lemma c4 : forall (n : nat) (k1 k2 : kind) (G : ctx)
+    (t1 : typ G (F k1 k2))
+    (t2 : typ G k1)
+    (envs : vec (env G) n),
+    zap (interp' t1 envs) (interp' t2 envs) = interp' (App t1 t2) envs.
+  Proof.
+    intros n k1 k2 G t1 t2 envs. generalize dependent G.
+    induction envs.
+    - destruct G.
+      + simpl. reflexivity.
+      + simpl. reflexivity.
+    -  destruct a.
+      + simpl. apply eqtail. unfold interp' in IHenvs. apply IHenvs.
+      + simpl. apply eqtail. unfold interp' in IHenvs. apply IHenvs.
+  Qed.
+
+  Lemma c3 : forall (n : nat) (k k' : kind) (G : ctx)
+    (t : typ (cons k' G) k) (envs : vec (env G) n) (As : vec (decodeKind k') n),
+    interp' t (zap (zap (repeat n (@econs k' G)) As) envs)
+    = zap (interp' (Lam t) envs) As.
+  Proof.
+    intros. destruct n.
+    - induction envs eqn:An.
+      + simpl. destruct G.
+        * simpl. reflexivity.
+        * simpl. reflexivity.
+      + destruct G.
+        * apply eqtail. simpl in IHv. apply IHv with (envs := v). reflexivity.
+        * apply eqtail. simpl. simpl in IHv. apply IHv with (envs := v). reflexivity.
+    - induction envs.
+      + simpl. destruct G.
+        * simpl. reflexivity.
+        * simpl. reflexivity.
+      + destruct G.
+        * apply eqtail. apply IHenvs.
+        * apply eqtail. apply IHenvs.
+  Qed.
+
+  Lemma c2 : forall (n : nat) (k k' : kind) (G : ctx)
+    (x : tyvar G k') (t1 : vec (decodeKind k) n) (envs : vec (env G) n),
+    interp' (Var x) envs
+    = interp' (Var (Vs _ x)) (zap (zap (repeat n (@econs _ _)) t1) envs).
+  Proof.
+    intros. induction envs.
+    - simpl. destruct G.
+      + simpl. reflexivity.
+      + simpl. reflexivity.
+    - simpl. destruct G.
+      + apply eqtail. apply IHenvs.
+      + apply eqtail. apply IHenvs.
+  Qed.
+
+  Lemma c1 : forall (n : nat) (k : kind) (G : ctx)
+    (a : vec (decodeKind k) n) (envs : vec (env G) n),
+    a = interp' (Var (Vz _ _)) (zap (zap (repeat n (@econs _ _)) a) envs).
+  Proof.
+    intros. induction a.
+    - simpl. reflexivity.
+    - apply eqtail. apply IHa.
+  Qed.
+
+  (* ADMITTED FOR TESTING OTHER DEFS *)
+  Fixpoint nlookup (n : nat) (k : kind) (b : vec Set (S n) -> Set) (G : ctx)
+    : forall (v : tyvar G k) (nge : ngenv b G),
+  kit k b (interp' (Var v) (transpose nge)). Admitted.
+
+  (*
+  Fixpoint nlookup' (n : nat) (k : kind) (b : vec Set (S n) -> Set) (G : ctx)
+    : forall (tv : tyvar G k) (nge : ngenv b G),
+    kit k b (interp' (Var tv) (transpose nge)) :=
+    fun tv nge =>
+      match tv in tyvar G k, nge in ngenv b G
+      return kit k b (interp' (Var tv) (transpose nge)) with
+      | Vz _ _, ncons _ x e ne =>
+          eqkit _ _ (c1 _ x (transpose ne))
+      | Vs g v, ncons _ x e ne =>
+          _
+    end.
+    *)
+
+  (* term specialization with non-empty context *)
+  Fixpoint ngen' (n : nat) (b : vec Set (S n) -> Set) (G : ctx) (k : kind) (t : typ G k)
+    : forall (ve : ngenv b G) (ce : tyConstEnv b), kit k b (interp' t (transpose ve)) :=
+    match t in typ G k
+    return forall (ve : ngenv b G) (ce : tyConstEnv b),
+    kit k b (interp' t (transpose ve)) with
+    | Var x => fun ve ce => nlookup x ve
+    | @Lam _ k1 k2 t1 => fun ve ce =>
+        curry _ (fun (a : vec (decodeKind k1) (S n)) (nwt : kit k1 b a) =>
+                  eqkit _ _ (c3 t1 (transpose ve) a)
+                  (ngen' t1 (ncons _ a nwt ve) ce))
+    | @App _ k1 k2 t1 t2 => fun ve ce =>
+        eqkit _ _ (c4 t1 t2 (transpose ve))
+        (@uncurry (S n) (decodeKind k1) (fun a => (forall _: kit k1 b a,
+                       (kit k2 b (zap (interp' t1 (transpose ve)) a))))
+        (@ngen' _ _ _ (F k1 k2) t1 ve ce)
+        (interp' t2 (transpose ve)) (ngen' t2 ve ce)
+        )
+    | Con _ c => fun ve ce => eqkit _ _ (c5 c (transpose ve)) (ce _ c)
+    end.
+
+  (* term specialization in an empty context. *)
+  Definition ngen (n : nat) (b : vec Set (S n) -> Set) (k : kind) (t : ty k)
+  (ce : tyConstEnv b) : kit k b (repeat (S n) (decodeClosed t)) :=
+  @eqkit n k b _ _ (c6 _ _ _ ) (ngen' t (nnil _) ce).
+
+End terms.
+
+(* generic map *)
+Definition gmap (k : kind) (t : ty k) : kit k Map (repeat 2 (decodeClosed t)) :=
+  ngen t mapConst.
+
+(* examples  of using gmap, still need to fix defs for 'nlookup' and 'uncurry' *)
+Compute gmap tprod _ _ (fun a => a + 1) _ _ (fun b => negb b) (1,true).
+(* tmaybe is a self defined type, definition in 'univ.v' *)
+Compute gmap tmaybe _ bool (fun _ => false) (inl tt). (* ~ Nothing *)
+Compute gmap tmaybe _ _ (fun _ => false) (inr 3). (* ~ Just 3 *)
+
